\documentclass{ximera}

\input{preamble.tex}

\author{Gregory Hartman \and Matthew Carr}
\license{Creative Commons 3.0 By-NC}
\acknowledgement{https://github.com/APEXCalculus}

\begin{document}
\begin{exercise}

\outcome{Calculate limits using the limit laws.}
\outcome{Calculate limits of the form 0/0.}
\outcome{Calculate limits using the Squeeze Theorem.}

\tag{limit} 
\tag{indeterminate form}
\tag{discontinuous}

% BADBAD 

It is a well known fact that $\lim_{x\to\infty}\left({\left({1+\frac{1}{x}}\right)^{x}}\right)=\lim_{x\to0}\left({(1+x)^{1/x}}\right)=e$.
Find 
\[
\lim_{x\to0}\left({\frac{\ln(1+x)}{x}}\right)
\begin{prompt}
= \answer{1}.
\end{prompt}
\]


\begin{hint}
Recall that $\lim_{x\to\infty}\left({\left({1+\frac{1}{x}}\right)^{x}}\right)=e$ and, equivalently, $\lim_{x\to0}\left({(1+x)^{1/x}}\right)=e$. Observe that we can rewrite this in a more illuminating way as $\frac{\ln(1+x)}{x}=x^{-1}\ln(1+x)$. Apply some properties of logarithms to this.
\end{hint}
\begin{hint}
We know, from the properties of logarithms, that $b\ln(a)=\ln({a^b})$ when $a>0$. Hence, $x^{-1}\ln(1+x)=\ln({(1+x)^{1/x}})$ for $x>-1$ (and, of course, $x^{-1}=\frac{1}{x}$). Hence, $\ln({(1+x)^{1/x}})=\frac{\ln(1+x)}{x}$ when $x\ne0$. So $\lim_{x\to0}\left(\ln({(1+x)^{1/x}})\right)=\lim_{x\to0}\left(\frac{\ln(1+x)}{x}\right)$. Recall that $\ln(x)$ is continuous everywhere besides $x=0$. What can you say about $\lim_{x\to0}\ln({(1+x)^{1/x}})$?
\end{hint}
\begin{hint}
Let $y=(1+x)^{1/x}$. Then, since $\lim_{x\to0}\left({(1+x)^{1/x}}\right)=e$, and $\ln(x)$ is continuous at $e$, it follows that $\lim_{x\to0}\left({\ln({(1+x)^{1/x}}})\right)=\lim_{y\to e}\left({\ln(y)}\right)=1$ and, hence, that $\lim_{x\to0}\left({\frac{\ln(1+x)}{x}}\right)=1$.
\end{hint}
\end{exercise}
\end{document}