\documentclass{ximera}

\input{../preamble.tex}

\author{Gregory Hartman \and Matthew Carr}
\license{Creative Commons 3.0 By-NC}
\acknowledgement{https://github.com/APEXCalculus}

\begin{document}
\begin{exercise}

\tag{derivative}

\outcome{Solve equations for $\frac{dy}{dx}$.}
\outcome{Implicitly differentiate expressions.}


Find the derivative $\frac{dy}{dx}$ if $\ln(x^2+xy+y^2)=1$.

\[
\frac{dy}{dx}
\begin{prompt}
= \answer{-\frac{2x+y}{2y+x}}
\end{prompt}
\]

\begin{hint}
Let $y$ be a function of $x$, $y(x)$. Then the chain rule tells us, for any function $f(y)$, that $\frac{d}{dx}f(y)=\left(\frac{d}{dy}\left(f(y)\right)\right)\left(\frac{dy}{dx}\right)$. 
\end{hint}

\begin{hint}
Applying the chain rule to the expression $\frac{d}{dx}(\ln(x^2+xy+y^2))=\frac{d}{dx}(1)=0$, we obtain $\frac{\frac{d}{dx}(x^2+xy+y^2)}{x^2+xy+y^2}=\frac{2x+y+x\frac{dy}{dx}+2y\frac{dy}{dx}}{x^2+xy+y^2}=0$. Solving for $\frac{dy}{dx}$, we obtain $\frac{dy}{dx}=-\frac{2x+y}{2y+x}$.
\end{hint}

\end{exercise}
\end{document}
