\documentclass{ximera}
%\input{../preamble.tex}
\author{Emma Smith Zbarsky}
\license{Creative Commons Attribution 3.0 Unported}
\acknowledgement{https://quadbase.org/questions/q13901v1}
\begin{document}

\begin{exercise}

Use the definition of the derivative to calculate
\[f'(t) = \frac{d}{dt}(f(t))\] for the function \[f(t) = 3t^2-2t+4.\]
You must write down the limit expression to evaluate as well as the
final derivative function.


\begin{hint}
Use the limit of the slopes of tangent lines passing through $(t,f(t))$
and $(t+\Delta t,f(t+\Delta t))$ as $\Delta t$ approaches zero to
calculate the derivative.
\end{hint}


\begin{hint}
The slope of the tangent line passing through $(t,f(t))$ and
$(t+\Delta t, f(t+\Delta t))$ is
\[\frac{\mbox{rise}}{\mbox{run}} = \frac{f(t+\Delta t) - f(t)}{(t+\Delta t)-t} = \frac{f(t+\Delta t)-f(t)}{\Delta t}.\]
The definition of the derivative says
\[f'(t) = \lim_{\Delta t \to 0} \frac{f(t+\Delta t)-f(t)}{\Delta t}.\]
Plugging in our function $f$ on the right hand side, this becomes
\begin{align*} f'(t) &= \lim_{\Delta t \to 0} \frac{3(t+\Delta t)^2-2(t+\Delta t)+4-3t^2+2t-4}{\Delta t} \\
&= \lim_{\Delta t \to 0} \frac{3t^2+6t\Delta t+3(\Delta t)^2-2t-2\Delta t+4-3t^2+2t-4}{\Delta t} \\
&= \lim_{\Delta t \to 0} \frac{6t\Delta t+3(\Delta t)^2-2\Delta t}{\Delta t} \\
&= \lim_{\Delta t \to 0} 6t-2 + 3\Delta t \\
&= \boxed{6t-2}
\end{align*}
\end{hint}


\begin{multipleChoice}
\choice[correct]{\begin{align*} f'(t) &= \lim_{\Delta t \to 0} \frac{3(t+\Delta t)^2-2(t+\Delta t)+4-3t^2+2t-4}{\Delta t} \\
&= \lim_{\Delta t \to 0} 6t-2 + 3\Delta t \\
&= \boxed{6t-2}
\end{align*}}
\choice{\begin{align*} f'(t) &= \lim_{\Delta t \to 0} \frac{3t^2+3(\Delta t)^2-2t-2\Delta t+4-3t^2+2t-4}{\Delta t} \\
&= \lim_{\Delta t \to 0} 6t-2 + 3\Delta t \\
&= \boxed{6t-2}
\end{align*}}
\choice{\begin{align*} f'(t) &= \lim_{\Delta t \to 0} \frac{3(t+\Delta t)^2-2(t+\Delta t)+4-3t^2+2t-4}{\Delta t} \\
&= \lim_{\Delta t \to 0} 6t-2 + 3\Delta t \\
&= \boxed{6t+1}
\end{align*}}
\choice{\begin{align*} f'(t) &= \lim_{\Delta t \to 0} \frac{3t^2+3(\Delta t)^2-2(t+\Delta t)+4-3t^2+2t-4}{\Delta t} \\
&= \lim_{\Delta t \to 0} -2 + 3\Delta t \\
&= \boxed{-2}
\end{align*}}
\end{multipleChoice}

\end{exercise}
\end{document}
