\documentclass{ximera}
%\input{../preamble.tex}
\author{Emma Smith Zbarsky}
\license{Creative Commons Attribution 3.0 Unported}
\acknowledgement{https://quadbase.org/questions/q14035v1}
\begin{document}

\begin{exercise}

Calculate the derivative of
\[f(\theta) = 3\cos(2\theta)-\frac{1}{2}\sin(5\theta)+\cos(3\pi).\]


\begin{hint}
This is a trignometric rule question with one constant rule component.
\end{hint}


\begin{hint}
First, notice that $\cos(3\pi) = -1$ is simply a constant, so by the
constant rule \[\frac{d}{d\theta}\left(\cos(3\pi)\right) = 0.\] Then you
need to remember that for any function $u(x)$ and any constant $a$,
\[\frac{d}{dx}\left(a\cos(u)\right) = -a\left(\frac{du}{dx}\right)\sin(u).\]
The negative goes along with derivatives of CO-functions: COsine,
COsecant, COtangent. Therefore,
\[\frac{d}{d\theta}\left(3\cos(2\theta)\right) = 3\left(\frac{d}{d\theta}\left(2\theta\right)\right)\left(-\sin(2\theta)\right) = -6\sin(2\theta).\]
Finally, you need to remember that for any function $u(x)$ and any
constant $a$,
\[\frac{d}{dx}\left(a\sin(u)\right) = a\left(\frac{du}{dx}\right)\cos(u).\]
Therefore,
\[\frac{d}{d\theta}\left(-\frac{1}{2}\sin(5\theta)\right) = -\frac{1}{2}\left(\frac{d}{d\theta}\left(5\theta\right)\right)\cos(5\theta) = -\frac{5}{2}\cos(5\theta).\]
Putting this together, we have:
\[\frac{d}{d\theta}\left(3\cos(2\theta)-\frac{1}{2}\sin(5\theta)+\cos(3\pi)\right) = -6\sin(2\theta)-\frac{5}{2}\sin(5\theta).\]
\end{hint}


\begin{multipleChoice}
\choice{$f'(\theta) = \frac{3}{2}\sin(2\theta)-\frac{1}{10}\cos(5\theta)-\theta$}
\choice[correct]{$f'(\theta) = -6\sin(2\theta)-\frac{5}{2}\cos(5\theta)$}
\choice{$f'(\theta) = -6\sin(2\theta)+\frac{5}{2}\cos(5\theta)-3\sin(3\pi)$}
\choice{$f'(\theta) = 6\sin(2\theta)-\frac{5}{2}\cos(5\theta)$}
\choice{$f'(\theta) = 6\sin(2\theta)+\frac{5}{2}\cos(5\theta)$}
\choice{$f'(\theta) = -6\sin(2\theta)+\frac{5}{2}\cos(5\theta)$}
\end{multipleChoice}

\end{exercise}
\end{document}
