\documentclass{ximera}
%\input{../preamble.tex}
\author{Emma Smith Zbarsky}
\license{Creative Commons Attribution 3.0 Unported}
\acknowledgement{https://quadbase.org/questions/q14027v1}
\begin{document}

\begin{exercise}

Calculate the derivative of the function \[y(t) = 4e^{-\frac{2}{5}t}.\]


\begin{hint}
This is an exponential rule problem.
\end{hint}


\begin{hint}
Solve this problem by applying the exponential rule--for any constants
$a$ and $b$ we have:
\[\frac{d}{dt}\left(ae^{bt}\right) = \frac{d(bt)}{dt}ae^{bt} = bae^{bt}.\]
Thus, with $a=4$ and $b=-\frac{2}{5}$ we have:
\[\frac{d}{dt}\left(4e^{-\frac{2}{5}t}\right) = -\frac{2}{5}\cdot 4 e^{-\frac{2}{5}t} = \boxed{-\frac{8}{5}e^{-\frac{2}{5}t}}.\]
\end{hint}


\begin{multipleChoice}
\choice{$y'(t) = -\frac{2}{5}e^{-\frac{2}{5}t}$}
\choice[correct]{$y'(t) = -\frac{8}{5}e^{-\frac{2}{5}t}$}
\choice{$y'(t) = \frac{8}{5}e^{-\frac{2}{5}t}$}
\choice{$y'(t) = -\frac{8}{5}te^{-\frac{2}{5}t}$}
\choice{$y'(t) = -\frac{5}{2}e^{-\frac{2}{5}t}$}
\end{multipleChoice}

\end{exercise}
\end{document}
