\documentclass{ximera}
%\input{../preamble.tex}
\author{Emma Smith Zbarsky}
\license{Creative Commons Attribution 3.0 Unported}
\acknowledgement{https://quadbase.org/questions/q14030v1}
\begin{document}

\begin{exercise}

Calculate the derivative of the function
\[y(t) = -\frac{1}{2}e^{\pi t}.\]


\begin{hint}
This is an exponential rule problem.
\end{hint}


\begin{hint}
Solve this problem by applying the exponential rule--for any constants
$a$ and $b$ we have:
\[\frac{d}{dt}\left(ae^{bt}\right) =\frac{d(bt)}{dt}ae^{bt} =  bae^{bt}.\]
Thus, with $a=-\frac{1}{2}$ and $b=\pi$ we have:
\[\frac{d}{dt}\left(-\frac{1}{2}e^{\pi t}\right) = \frac{d(\pi t)}{dt} \left(-\frac{1}{2} e^{\pi t}\right) = \boxed{-\frac{\pi}{2}e^{\pi t}}.\]
\end{hint}


\begin{multipleChoice}
\choice{$y'(t) = \pi e^{-\pi/2 t}$}
\choice{$y'(t) = -\frac{\pi}{2}te^{\pi t}$}
\choice{$y'(t) = -\frac{\pi}{2}te^{\pi t-1}$}
\choice{$y'(t) = -\frac{1}{2\pi}e^{\pi t}$}
\choice[correct]{$y'(t) = -\frac{\pi}{2}e^{\pi t}$}
\end{multipleChoice}

\end{exercise}
\end{document}
