\documentclass{ximera}
%\input{../preamble.tex}
\author{Emma Smith Zbarsky}
\license{Creative Commons Attribution 3.0 Unported}
\acknowledgement{https://quadbase.org/questions/q14020v1}
\begin{document}

\begin{exercise}

Calculate the derivative of the function
\[f(x) = 3x^7+\frac{1}{2}x^{2/3}-5x+1.\]


\begin{hint}
This is a power rule question.
\end{hint}


\begin{hint}
Solve this using the power rule applied to each term--for any constants
$a$ and $n \neq 0$: \[\frac{d}{dx}\left(ax^n\right) = nax^{n-1}.\] If
$n=0$ we call this the constant rule:\[\frac{d}{dx}\left(a\right) = 0.\]
\begin{align*}
\frac{d}{dx}(3x^7) &= 7\cdot 3x^6 = 21x^6 \\
\frac{d}{dx}\left(\frac{1}{2}x^{2/3}\right) &= \frac{2}{3}\cdot \frac{1}{2}x^{2/3-1} = \frac{1}{3}x^{-1/3} \\
\frac{d}{dx}(-5x) &= -5 \\
\frac{d}{dx}(1) &= 0 \\
\end{align*}

Putting the pieces together, we see that
\[\frac{d}{dx}\left(3x^7+\frac{1}{2}x^{2/3}-5x+1\right) = \boxed{21x^6+\frac{1}{3}x^{-1/3}-5}.\]
\end{hint}


\begin{multipleChoice}
\choice{$f'(x) = \frac{3}{8}x^8+\frac{3}{10}x^{5/3}-\frac{5}{2}x^2+x$}
\choice{$f'(x) = 21x^6+\frac{1}{3}x^{1/3}-5$}
\choice[correct]{$f'(x) = 21x^6+\frac{1}{3}x^{-1/3}-5$}
\choice{$f'(x) = 21x^6+\frac{3}{4}x^{5/3}-5$}
\choice{$f'(x) = 7x^6+x^{-1/3}-1$}
\end{multipleChoice}

\end{exercise}
\end{document}
