\documentclass{ximera}
%\input{../preamble.tex}
\author{Emma Smith Zbarsky}
\license{Creative Commons Attribution 3.0 Unported}
\acknowledgement{https://quadbase.org/questions/q14025v1}
\begin{document}

\begin{exercise}

Calculate the derivative of the function \[y(t) = 8e^{-3t}.\]


\begin{hint}
This is an exponential rule problem.
\end{hint}


\begin{hint}
Solve this problem by applying the exponential rule--for any constants
$a$ and $b$ we have:
\[\frac{d}{dt}\left(ae^{bt}\right) = \frac{d(bt)}{dt}ae^{bt} = bae^{bt}.\]
Thus, with $a=8$ and $b=-3$ we have:
\[\frac{d}{dt}\left(8e^{-3t}\right) = -3\cdot 8 e^{-3t} = \boxed{-24e^{-3t}}.\]
\end{hint}


\begin{multipleChoice}
\choice[correct]{$y'(t) = -24e^{-3t}$}
\choice{$y'(t) = -\frac{8}{3}e^{-3t}$}
\choice{$y'(t) = -3e^{-3t}$}
\choice{$y'(t) = -24t e^{-3t-1}$}
\choice{$y'(t) = 8e^{-3t}$}
\end{multipleChoice}

\end{exercise}
\end{document}
