\documentclass{ximera}
%\input{../preamble.tex}
\author{Emma Smith Zbarsky}
\license{Creative Commons Attribution 3.0 Unported}
\acknowledgement{https://quadbase.org/questions/q14282v1}
\begin{document}

\begin{exercise}

Calculate the derivative of $V(r)$ with respect to $r$ if
\[V(r) = \ln\left((3r-5)e^{2r}\right).\]


\begin{hint}
This is a log rule problem which simplifies immensely if you apply your
algebraic log rules before attempting the calculus. In particular, you
should use $\ln(MN) = \ln(M)+\ln(N)$
\end{hint}


\begin{hint}
Rewriting, we have
\[V(r) = \ln\left((3r-5)e^{2r}\right) = \ln(3r-5)+\ln\left(e^{2r}\right) = \ln(3r-5)+2r.\]
Then taking the derivative we have \begin{align*}
V'(r) &= \frac{1}{3r-5}\frac{d}{dr}\left(3r-5\right) +2 \\
&= \frac{3}{3r-5}+2
\end{align*}

If you do not simplify before taking the derivative, we have
\begin{align*}
V'(r) &= \frac{1}{(3r-5)e^{2r}}\frac{d}{dr}\left((3r-5)e^{2r}\right) \\
&= \frac{3e^{2r}+2(3r-5)e^{2r}}{(3r-5)e^{2r}} \\
&= \frac{3}{3r-5} + 2
\end{align*}
\end{hint}


\begin{multipleChoice}
\choice{$V'(r) = \ln\left((3r-5)e^{2r}\right)$}
\choice{$V'(r) = \frac{3}{(3r-5)e^{2r}}$}
\choice{$V'(r) = (6r-7)e^{2r}\ln\left((3r-5)e^{2r}\right)$}
\choice{$V'(r) = \frac{1}{(3r-5)e^{2r}}$}
\choice[correct]{$V'(r) = \frac{3}{3r-5}+2$}
\end{multipleChoice}

\end{exercise}
\end{document}
