\documentclass{ximera}
%\input{../preamble.tex}
\author{Emma Smith Zbarsky}
\license{Creative Commons Attribution 3.0 Unported}
\acknowledgement{https://quadbase.org/questions/q14277v1}
\begin{document}

\begin{exercise}

Calculate the derivative $\frac{df}{dx}$ with
\[f(x) = x\csc(3x^2-2x+8).\]


\begin{hint}
This problem uses both the chain rule and the product rule, as well as
derivatives of basic functions.
\end{hint}


\begin{hint}
If we use $\frac{d}{dx}(ab) = a'b+b'a$ for the product rule, then $a=x$
and $b=\csc(3x^2-2x+8)$. Then, $a'=1$ is easy, but to calculate $b'$ we
also need the chain rule,
$\frac{d}{dx}\left(f(g(x))\right) = \frac{df}{dg}\cdot\frac{dg}{dx}$
where we identify \begin{align*}
g &= \csc(u) \Rightarrow \frac{dg}{du} = -\csc(u)\cot(u) \\
u &= 3x^2-2x+8 \Rightarrow \frac{du}{dx} = 6x-2 \\
b' &= \frac{d}{dx}(g(u(x))) = -\csc(3x^2-2x+8)\cot(3x^2-2x+8)(6x-2)\\
\end{align*} Putting this all together we have
\[f'(x) = \csc(3x^2-2x+8)-(6x^2-2x)\csc(3x^2-2x+8)\cot(3x^2-2x+8)\]
\end{hint}


\begin{multipleChoice}
\choice{$f'(x) = \csc(3x^2-2x+8)-x\csc(6x-2)\cot(6x-2)$}
\choice{$f'(x) = \csc(3x^2-2x+8)+x\csc(6x-2)\cot(6x-2)$}
\choice{$f'(x) = (6x^2-2x)\csc(3x^2-2x+8)\cot(3x^2-2x+8)$}
\choice[correct]{$f'(x) = \csc(3x^2-2x+8) - (6x^2-2x)\csc(3x^2-2x+8)\cot(3x^2-2x+8)$}
\choice{$f'(x) = \csc(3x^2-2x+8) + (6x^2-2x)\csc(3x^2-2x+8)\cot(3x^2-2x+8)$}
\end{multipleChoice}

\end{exercise}
\end{document}
