\documentclass{ximera}
%\input{../preamble.tex}
\author{Emma Smith Zbarsky}
\license{Creative Commons Attribution 3.0 Unported}
\acknowledgement{https://quadbase.org/questions/q14230v1}
\begin{document}

\begin{exercise}

Calculate the derivative of \[h(t) = \tan(t)e^t.\]


\begin{hint}
This is a product rule question. You need to use
\[\frac{d}{dt}\left(f(t)g(t)\right) = f'(t)g(t)+f(t)g'(t)\] to solve it.
\end{hint}


\begin{hint}
Using the product rule,
\[\frac{d}{dt}\left(f(t)g(t)\right) = f'(t)g(t)+f(t)g'(t),\] and
$f(t) = \tan(t),$ $g(t) = e^t$ we have
\begin{align*} \frac{d}{dt}\left(\tan(t)e^t\right) &= \frac{d}{dt}\left(\tan(t)\right)e^t+\tan(t)\left(\frac{d}{dt}\left(e^t\right)\right) \\
&= \boxed{\sec^2(t)e^t + \tan(t)e^t}
\end{align*}
\end{hint}


\begin{multipleChoice}
\choice{$h'(t) = \tan(t)e^t$}
\choice{$h'(t) = \sec^2(t)e^t+t\tan(t)e^{t-1}$}
\choice[correct]{$h'(t) = \sec^2(t)e^t+\tan(t)e^t$}
\choice{$h'(t) = 2\sec(t)e^t+\tan(t)e^t$}
\choice{$h'(t) = \sec^2(t)+e^t$}
\end{multipleChoice}

\end{exercise}
\end{document}
