\documentclass{ximera}
%\input{../preamble.tex}
\author{Emma Smith Zbarsky}
\license{Creative Commons Attribution 3.0 Unported}
\acknowledgement{https://quadbase.org/questions/q14227v1}
\begin{document}

\begin{exercise}

Calculate the derivative of \[g(x) = 3x^2e^x.\]


\begin{hint}
This is a product rule question. You need to use
\[\frac{d}{dx}\left(f(x)g(x)\right) = f'(x)g(x)+f(x)g'(x)\] to solve it.
\end{hint}


\begin{hint}
Using the product rule,
\[\frac{d}{dx}\left(f(x)g(x)\right) = f'(x)g(x)+f(x)g'(x),\] we have
\begin{align*} \frac{d}{dx}\left(3x^2e^x\right) &= \frac{d}{dx}\left(3x^2\right)e^x + 3x^2\left(\frac{d}{dx}\left(e^x\right)\right) \\
&= \left(6x\right)e^x + 3x^2\left(e^x\right) \\
&= \boxed{6xe^x+3x^2e^x}
\end{align*}
\end{hint}


\begin{multipleChoice}
\choice{$g'(x) = 6xe^x + 3e^x$}
\choice{$g'(x) = 3+6x+e^x$}
\choice{$g'(x) = 6xe^x$}
\choice{$g'(x) = 2xe^x + 3x^2e^x$}
\choice[correct]{$g'(x) = 6xe^x+3x^2e^x$}
\end{multipleChoice}

\end{exercise}
\end{document}
