\documentclass{ximera}
%\input{../preamble.tex}
\author{Emma Smith Zbarsky}
\license{Creative Commons Attribution 3.0 Unported}
\acknowledgement{https://quadbase.org/questions/q14278v1}
\begin{document}

\begin{exercise}

Calculate the derivative of $y(t)$ with respect to $t$ if
\[y(t) = \sec(4t-5)e^{\frac{7}{3}t}.\]


\begin{hint}
This is a mixed rule derivative problem involving both product rule and
chain rule, as well as our basic derivatives of functions.
\end{hint}


\begin{hint}
If we identify $y(t) = a(t)b(t)$ for the product rule with
$a(t) = \sec(4t-5)$ and $b(t) = e^{\frac{7}{3}t}$, and $a(t) = f(g(t))$
for the chain rule with $f(g) = \sec(g)$ and $g(t) = 4t-5$ we have:
\begin{align*}
y'(t) &= \frac{d}{dt}\left(sec(4t-5)\right)e^{\frac{7}{3}t} + \sec(4t-5)\frac{d}{dt}\left(e^{\frac{7}{3}t}\right) \\
&= \left(\sec(4t-5)\tan(4t-5)\frac{d}{dt}(4t-5)\right)e^{\frac{7}{3}t} + \sec(4t-5)\left(\frac{7}{3}e^{\frac{7}{3}t}\right) \\
&= 4\sec(4t-5)\tan(4t-5)e^{\frac{7}{3}t} + \frac{7}{3}\sec(4t-5)e^{\frac{7}{3}t} \\
&= \left(4\tan(4t-5)+\frac{7}{3}\right)\sec(4t-5)e^{\frac{7}{3}t}
\end{align*}
\end{hint}


\begin{multipleChoice}
\choice{$y'(t) = 4\sec(4t-5)\tan(4t-5)e^{\frac{7}{3}t}$}
\choice[correct]{$y'(t) = \left(4\tan(4t-5)+\frac{7}{3}\right)\sec(4t-5)e^{\frac{7}{3}t}$}
\choice{$y'(t) = \frac{28}{3}\sec(4t-5)\tan(4t-5)e^{\frac{7}{3}t}$}
\choice{$y'(t) = \sec(4t-5)\tan(4t-5)e^{\frac{7}{3}t}$}
\choice{$y'(t) = \left(4\tan(4t-5)-\frac{7}{3}\right)\sec(4t-5)e^{\frac{7}{3}t}$}
\end{multipleChoice}

\end{exercise}
\end{document}
