\documentclass{ximera}
%\input{../preamble.tex}
\author{Emma Smith Zbarsky}
\license{Creative Commons Attribution 3.0 Unported}
\acknowledgement{https://quadbase.org/questions/q14259v1}
\begin{document}

\begin{exercise}

Calculate the derivative with respect to $t$ of
\[g(t) = \frac{4}{3}t^3e^{3t}\cos(3t).\]


\begin{hint}
This is a product rule question, but you will need to split the problem
up more than once.
\end{hint}


\begin{hint}
For instance, we could calculate:

\begin{align*}
g'(t) &= \frac{d}{dt}\left(\frac{4}{3}t^3\right)e^{3t}\cos(3t) + \frac{4}{3}t^3\frac{d}{dt}\left(e^{3t}\cos(3t)\right) \\
&= 4t^2e^{3t}\cos(3t) + \frac{4}{3}t^3\left(\frac{d}{dt}\left(e^{3t}\right)\cos(3t) + e^{3t}\frac{d}{dt}\left(\cos(3t)\right)\right) \\
&= 4t^2e^{3t}\cos(3t) + \frac{4}{3}t^3\left(3e^{3t}\cos(3t)-3e^{3t}\sin(3t)\right) \\
&= 4t^2e^{3t}\cos(3t)+4t^3e^{3t}\cos(3t)-4t^3e^{3t}\sin(3t) \\
&= e^{3t}\left((4t^2+4t^3)\cos(3t)-4t^3\sin(3t)\right)
\end{align*}
\end{hint}


\begin{multipleChoice}
\choice[correct]{$g'(t) = e^{3t}\left((4t^2+4t^3)\cos(3t)-4t^3\sin(3t)\right)$}
\choice{$g'(t) = 4t^2e^{3t}\cos(3t)-4t^3e^{3t}\sin(3t)$}
\choice{$g'(t) = -3t^2e^{3t}\sin(3t)$}
\choice{$g'(t) = 4t^2\left(e^{3t}\cos(3t)- te^{3t}\sin(3t)\right)$}
\choice{$g'(t) = 4\left(t^2+e^{3t}-\sin(3t)\right)$}
\end{multipleChoice}

\end{exercise}
\end{document}
