\documentclass{ximera}
%\input{../preamble.tex}
\author{Emma Smith Zbarsky}
\license{Creative Commons Attribution 3.0 Unported}
\acknowledgement{https://quadbase.org/questions/q14257v1}
\begin{document}

\begin{exercise}

Calculate the derivative with respect to $x$ of
\[f(x) = \frac{e^{x}+2e^{-x}}{\tan(3x)+2}.\]


\begin{hint}
This is a quotient rule problem. You need to use
\[\frac{d}{dx}\left(\frac{p(x)}{q(x)}\right) = \frac{p'(x)q(x)-p(x)q'(x)}{(q(x))^2}.\]
\end{hint}


\begin{hint}
Let $p(x) = e^x+2e^{-x}$ and $q(x) = \tan(3x)+2$. Then \begin{align*}
p'(x) &= e^x-2e^{-x} \\
q'(x) &= 3\sec^2(3x) \\
f'(x) &= \frac{\left(e^x-2e^{-x}\right)\left(\tan(3x)+2\right) - \left(e^x+2e^{-x}\right)\left(3\sec^2(3x)\right)}{\left(\tan(3x)+2\right)^2} \\
&= \frac{\left(e^x-2e^{-x}\right)\left(\tan(3x)+2\right) - 3\left(e^x+2e^{-x}\right)\sec^2(3x)}{\left(\tan(3x)+2\right)^2}
\end{align*}
\end{hint}


\begin{multipleChoice}
\choice{$f'(x) = \frac{(e^x-2e^{-x})(\tan(3x)+2)-(e^x-2e^{-x})\sec^2(3x)}{(\tan(3x)+2)^2}$}
\choice{$f'(x) = \frac{(e^x-2e^{-x})(\tan(3x)+2)-3(e^x+2e^{-x})\sec^2(3x)}{\tan(3x)+2}$}
\choice{$f'(x) = \frac{e^x-2e^{-x}}{3\sec^2(3x)}$}
\choice[correct]{$f'(x) = \frac{(e^x-2e^{-x})(\tan(3x)+2)-3(e^x+2e^{-x})\sec^2(3x)}{(\tan(3x)+2)^2}$}
\choice{$f'(x) = \frac{-(e^x-2e^{-x})(\tan(3x)+2)+3(e^x+2e^{-x})\sec^2(3x)}{(\tan(3x)+2)^2}$}
\end{multipleChoice}

\end{exercise}
\end{document}
