\documentclass{ximera}
%\input{../preamble.tex}
\author{Emma Smith Zbarsky}
\license{Creative Commons Attribution 3.0 Unported}
\acknowledgement{https://quadbase.org/questions/q14283v1}
\begin{document}

\begin{exercise}

Calculate the derivative with respect to $x$ of
\[Q(x) = \ln\left(\frac{3x-5}{6x^2+7x-2}\right).\]


\begin{hint}
This is a logarithm rule problem, and, as usual, benefits from algebraic
simplification before you start in on the calculus.
\end{hint}


\begin{hint}
\begin{align*}
Q(x) &= \ln\left(\frac{3x-5}{6x^2+7x-2}\right) \\
&= \ln(3x-5)-\ln(6x^2+7x-2) \\
Q'(x) &= \frac{1}{3x-5}\frac{d}{dx}(3x-5) - \frac{1}{6x^2+7x-2}\frac{d}{dx}\left(6x^2+7x-2\right) \\
&=\frac{3}{3x-5} - \frac{12x+7}{6x^2+7x-2}
\end{align*}
\end{hint}


\begin{multipleChoice}
\choice{$Q'(x) = \frac{1}{3x-5} - \frac{1}{6x^2+7x-2}$}
\choice{$Q'(x) = \frac{6x^2+7x-2}{3x-5}$}
\choice{$Q'(x) = \frac{3}{3x-5} + \frac{12x+7}{6x^2+7x-2}$}
\choice[correct]{$Q'(x) = \frac{3}{3x-5} - \frac{12x+7}{6x^2+7x-2}$}
\choice{$Q'(x) = \frac{1}{3x-5}+\frac{1}{6x^2+7x-2}$}
\end{multipleChoice}

\end{exercise}
\end{document}
