\documentclass{ximera}
%\input{../preamble.tex}
\author{Emma Smith Zbarsky}
\license{Creative Commons Attribution 3.0 Unported}
\acknowledgement{https://quadbase.org/questions/q14252v1}
\begin{document}

\begin{exercise}

Calculate the derivative with respect to $t$ of
\[f(t) = (3t-4)(t^2-1).\]


\begin{hint}
This is easy as a product rule question, because then the multiplication
is simple.
\end{hint}


\begin{hint}
Using \[\frac{d}{dt}\left(f(t)g(t)\right) = f'(t)g(t)+f(t)g'(t),\] with
$f(t) = 3t-4$ and $g(t) = t^2-1$ we have \[f'(t) = 3\] and
\[g'(t) = 2t\] so
\begin{align*}\frac{d}{dt}\left((3t-4)(t^2-1)\right) &= 3(t^2-1)+(3t-4)(2t) \\ &= 3t^2-3+6t^2-8t \\ &= \boxed{9t^2-8t-3}\end{align*}
\end{hint}


\begin{multipleChoice}
\choice{$f'(t) = 3t^2-3$}
\choice{$f'(t) = 6t^2-8t-3$}
\choice{$f'(t) = 6t^2-8t$}
\choice[correct]{$f'(t) = 9t^2-8t-3$}
\choice{$f'(t) = -2t-3$}
\end{multipleChoice}

\end{exercise}
\end{document}
