\documentclass{ximera}
%\input{../preamble.tex}
\author{Emma Smith Zbarsky}
\license{Creative Commons Attribution 3.0 Unported}
\acknowledgement{https://quadbase.org/questions/q14231v1}
\begin{document}

\begin{exercise}

Calculate the derivative $\frac{dy}{dt}$ of
\[y(t) = \frac{3t-2}{6t^2+12t+6}.\]


\begin{hint}
This is a quotient rule problem. You will need to use
\[\frac{d}{dt}\left(\frac{p(t)}{q(t)}\right) = \frac{p'(t)q(t)-p(t)q'(t)}{\left(q(t)\right)^2}\]
to solve it.
\end{hint}


\begin{hint}
Using
$\frac{d}{dt}\left(\frac{p(t)}{q(t)}\right) = \frac{p'(t)q(t)-p(t)q'(t)}{\left(q(t)\right)^2},$
with $p(t) = 3t-2$ and $q(t) = 6t^2+12t+6$ we see that \begin{align*}
y'(t) &= \frac{3(6t^2+12t+6)-(3t-2)(12t+12)}{(6t^2+12t+6)^2} \\
&= \frac{(18t^2+36t+18)-(36t^2-24t+36t-24)}{(6t^2+12t+6)^2} \\
&= \frac{-18t^2+24t+42}{(6t^2+12t+6)^2} \\
&= \boxed{\frac{-3t^2+4t+7}{6(t^2+2t+1)^2}}
\end{align*}
\end{hint}


\begin{multipleChoice}
\choice{$y'(t) = \frac{-3t^2+4t+7}{(t^2+2t+1)^2}$}
\choice{$y'(t) = \frac{-3t^2+4t-1}{t^2+2t+1}$}
\choice{$y'(t) = \frac{-3t^2+4t-1}{6(t^2+2t+1)^2}$}
\choice{$y'(t) = \frac{-3t^2+2t-1}{6(t^2+2t+1)^2}$}
\choice[correct]{$y'(t) = \frac{-3t^2+4t+7}{6(t^2+2t+1)^2}$}
\end{multipleChoice}

\end{exercise}
\end{document}
