\documentclass{ximera}
%\input{../preamble.tex}
\author{Emma Smith Zbarsky}
\license{Creative Commons Attribution 3.0 Unported}
\acknowledgement{https://quadbase.org/questions/q14267v1}
\begin{document}

\begin{exercise}

Calculate the derivative with respect to $v$ of
\[G(v) = e^{5v^2+2v-3}.\]


\begin{hint}
This is a chain rule problem. You need to use
\[\frac{d}{dv}f(g(v)) = \frac{df}{dg}\cdot\frac{dg}{dv}.\]
\end{hint}


\begin{hint}
Let $f(g) = e^g$ and $g(v) = 5v^2+2v-3$. Then we have \begin{align*}
\frac{df}{dg} &= e^g \\
\frac{dg}{dv} &= 10v+2 \\
\frac{d}{dv}\left(f(g(v))\right) &= \frac{d}{dv}\left(e^{5v^2+2v-3}\right) \\
&= e^g(10v+2) \\ &= \boxed{(10v+2)e^{5v^2+2v-3}}
\end{align*}
\end{hint}


\begin{multipleChoice}
\choice{$G'(v) = (5v^2+2v-3)e^{5v^2+2v-3}$}
\choice[correct]{$G'(v) = (10v+2)e^{5v^2+2v-3}$}
\choice{$G'(v) = e^{5v^2+2v-3}$}
\choice{$G'(v) = e^{10v+2}$}
\choice{$G'(v) = (10v+2)e^{5v^2+2v-4}$}
\end{multipleChoice}

\end{exercise}
\end{document}
