\documentclass{ximera}
%\input{../preamble.tex}
\author{Emma Smith Zbarsky}
\license{Creative Commons Attribution 3.0 Unported}
\acknowledgement{https://quadbase.org/questions/q14269v1}
\begin{document}

\begin{exercise}

Calculate the derivative with respect to $t$ of
\[P(t) = \left(4t+e^{6t-4}-\sec(3t/2)\right)^5.\]


\begin{hint}
This is a chain rule problem. You need to remember that
\[\frac{d}{dt}\left(f(g(t))\right) = f'(g)g'(t) = \frac{df}{dg}\cdot\frac{dg}{dt}.\]
\end{hint}


\begin{hint}
Consider the given function
$P(t)=\left(4t+e^{6t-4}-\sec(3t/2)\right)^5$, and remember to use
parentheses as your guide. Thus, we see that this function is
$P(t) = f(g(t))$ for $f(g) = g^5$ and $g(t) = 4t+e^{6t-4}-\sec(3t/2)$.
This gives us \begin{align*}
\frac{df}{dg} &= 5g^4 \\
\frac{dg}{dt} &= 4+6e^{6t-4}-\frac{3}{2}\sec(3t/2)\tan(3t/2) \\
P'(t) &= 5\left(4t+e^{6t-4}-\sec(3t/2)\right)^4\left(4+6e^{6t-4}-\frac{3}{2}\sec(3t/2)\tan(3t/2)\right)
\end{align*}
\end{hint}


\begin{multipleChoice}
\choice{$P'(t) = 5\left(4t+e^{6t-4}-\sec(3t/2)\right)^4\left(4+6te^{5t-4}-\frac{3}{2}\sec(3t/2)\tan(3t/2)\right)$}
\choice{$P'(t) = 5\left(4t+e^{6t-4}-\sec(3t/2)\right)^4\left(4+6e^{6t-4}+\frac{3}{2}\sec(3t/2)\tan(3t/2)\right)$}
\choice[correct]{$P'(t) = 5\left(4t+e^{6t-4}-\sec(3t/2)\right)^4\left(4+6e^{6t-4}-\frac{3}{2}\sec(3t/2)\tan(3t/2)\right)$}
\choice{$P'(t) = 5\left(4t+e^{6t-4}-\sec(3t/2)\right)^4$}
\choice{$P'(t) = 5\left(4+6e^{6t-4}-\frac{3}{2}\sec(3t/2)\tan(3t/2)\right)^4$}
\end{multipleChoice}

\end{exercise}
\end{document}
