\documentclass{ximera}
%\input{../preamble.tex}
\author{Emma Smith Zbarsky}
\license{Creative Commons Attribution 3.0 Unported}
\acknowledgement{https://quadbase.org/questions/q14281v1}
\begin{document}

\begin{exercise}

Calculate the derivative $\frac{dq}{dt}$ if \[q(t) = \ln(t^2-2t+1).\]


\begin{hint}
This is a log rule problem. It is frequently useful to apply algebraic
log rules before attempting calculus. In this case, the problem
simplifies if you note that
\[\ln(t^2-2t+1) = \ln\left((t-1)^2\right) = 2\ln(t-1).\]
\end{hint}


\begin{hint}
Using the above simplification, the derivative becomes: \begin{align*}
q'(t) &= 2\frac{d}{dt}\left(\ln(t-1)\right) \\
&= 2 \left(\frac{1}{t-1}\right)\frac{d}{dt}\left(t-1\right) \\
&= \frac{2}{t-1}
\end{align*} However, if you do not notice the algebraic
simplification initially, you will find the same answer by plowing
through: \begin{align*}
q'(t) &= \frac{1}{t^2-2t+1}\frac{d}{dt}\left(t^2-2t+1\right) \\
&= \frac{2t-2}{t^2-2t+1} \\
&= \frac{2(t-1)}{(t-1)^2} \\
&= \frac{2}{t-1}
\end{align*}
\end{hint}


\begin{multipleChoice}
\choice[correct]{$q'(t) = \frac{2}{t-1}$}
\choice{$q'(t) = \frac{t-1}{\ln(t-1)}$}
\choice{$q'(t) = (2t-2)\ln(t^2-2t+1)$}
\choice{$q'(t) = \ln(t^2-2t+1)$}
\choice{$q'(t) = \frac{1}{t^2-2t+1}$}
\end{multipleChoice}

\end{exercise}
\end{document}
