\documentclass{ximera}
%\input{../preamble.tex}
\author{Emma Smith Zbarsky}
\license{Creative Commons Attribution 3.0 Unported}
\acknowledgement{https://quadbase.org/questions/q14352v1}
\begin{document}

\begin{exercise}

Use implicit differentiation to calculate $\frac{dx}{dt}$ if
\[x^3t^2 = 6xt-3.\]


\begin{hint}
This is an implicit differentiation problem. You need to treat each $x$
as a function $x(t)$ and use the product and chain rules appropriately.
Take the derivative $\frac{d}{dt}$ of both sides and then solve for the
$\frac{dx}{dt}$ that arises from using the chain rule.
\end{hint}


\begin{hint}
\begin{align*}
\frac{d}{dt}\left(x^3t^2\right) &= \frac{d}{dt}\left(6xt-3\right) \\
3x^2t^2\frac{dx}{dt}+2x^3t &= 6t\frac{dx}{dt} + 6x \\
\frac{dx}{dt}\left(3x^2t^2-6t\right) &= 6x-2x^3t \\
\frac{dx}{dt} &= \frac{6x-2x^3t}{3x^2t^2-6t} 
\end{align*}
\end{hint}


\begin{multipleChoice}
\choice[correct]{$\frac{dx}{dt} = \frac{6x-2x^3t}{3x^2t^2-6t}$}
\choice{$\frac{dx}{dt} = 6x-2x^3t$}
\choice{$\frac{dx}{dt} = \frac{3x^2t^2-6t}{6x-2x^3t}$}
\choice{$\frac{dx}{dt} = \frac{6t+6x-2x^3t}{3x^2t^2}$}
\choice{$\frac{dx}{dt} = \frac{3x^2t^2+2x^3t-6x}{6t}$}
\end{multipleChoice}

\end{exercise}
\end{document}
