\documentclass{ximera}
%\input{../preamble.tex}
\author{Emma Smith Zbarsky}
\license{Creative Commons Attribution 3.0 Unported}
\acknowledgement{https://quadbase.org/questions/q14350v1}
\begin{document}

\begin{exercise}

Use implicit differentiation to calculate $\frac{dy}{dx}$ in terms of
$x$ and $y$ for an ellipse with \[3y^2+2x^2 = 4.\]


\begin{hint}
This is an implicit differentiation problem. You need to treat each $y$
as a function $y(x)$ and use the product and chain rules appropriately.
Take the derivative $\frac{d}{dx}$ of both sides and then solve for the
$\frac{dy}{dx}$ that arises from using the chain rule.
\end{hint}


\begin{hint}
\begin{align*}
\frac{d}{dx}\left(3y^2+2x^2\right) &= \frac{d}{dx}(4) \\
3\frac{d}{dx}\left(y^2\right) + 2\frac{d}{dx}\left(x^2\right) &= 0 \\
3\left(2y\right)\frac{dy}{dx} + 2\left(2x\right) &= 0 \\
6y\frac{dy}{dx} &= -4x \\
\frac{dy}{dx} &= -\frac{4x}{6y} = -\frac{2x}{3y}
\end{align*}
\end{hint}


\begin{multipleChoice}
\choice{$\frac{dy}{dx} = -6y-4x$}
\choice[correct]{$\frac{dy}{dx} = -\frac{2x}{3y}$}
\choice{$\frac{dy}{dx} = \frac{2x}{3y}$}
\choice{$\frac{dy}{dx} = 6y+4x$}
\choice{$\frac{dy}{dx} = 4x$}
\end{multipleChoice}

\end{exercise}
\end{document}
