\documentclass{ximera}
%\input{../preamble.tex}
\author{Emma Smith Zbarsky}
\license{Creative Commons Attribution 3.0 Unported}
\acknowledgement{https://quadbase.org/questions/q14518v1}
\begin{document}

\begin{exercise}

Find the function $x(t)$ that satisfies $x'(t) = 4e^{-7t}+6$ with
$x(0)=\frac{3}{7}$.


\begin{hint}
This is an initial value problem. Find the general antiderivative of
$x'(t)$, then use the initial condition given to solve for the
particular antiderivative requested.
\end{hint}


\begin{hint}
\begin{align*}
x'(t) &= 4e^{-7t}+6 \\
\int x'(t) \; dt &= \int 4e^{-7t}+6\; dt \\
x(t) &= -\frac{4}{7}e^{-7t}+6t+C \\
x(0) = \frac{3}{7} &= -\frac{4}{7}e^{-7(0)}+6(0)+C \\
&\Rightarrow C=1 \\
x(t) &= -\frac{4}{7}e^{-7t}+6t+1 \end{align*}
\end{hint}


\begin{multipleChoice}
\choice[correct]{$x(t) = -\frac{4}{7}e^{-7t}+6t+1$}
\choice{$x(t) = -28e^{-7t}+6t+\frac{199}{7}$}
\choice{$x(t) = \frac{4}{7}e^{-7t}+1$}
\choice{$x(t) = -\frac{4}{7}e^{-7t}+6t+\frac{3}{7}$}
\choice{$x(t) = \frac{4}{7}e^{-7t}+6t-\frac{1}{7}$}
\end{multipleChoice}

\end{exercise}
\end{document}
