\documentclass{ximera}
\input{../preamble.tex}
\author{Steven Gubkin}
\license{Creative Commons 3.0 By-NC}
\begin{document}
\begin{exercise}


\tag{integral}

Find the area of the region bounded by the curves $y=x-2$ and $y=-x$, and $y = 4+2x-x^2$.

\begin{hint}

	First sketch a picture of the region

\begin{image}
\begin{tikzpicture}
	\begin{axis}[
            domain=-2:5, ymax=5,xmax=5,ymin=-2, xmin=-2,
            axis lines =center, xlabel=$x$, ylabel=$y$,
 	   xtick={-1,1,3},
            xticklabels={$a$,$b$,$c$}, 
            every axis y label/.style={at=(current axis.above origin),anchor=south},
            every axis x label/.style={at=(current axis.right of origin),anchor=west},
            axis on top,
          ]
          \addplot [draw=none,fill=fillp,domain=-1:3] {4+2*x-x^2} \closedcycle;
          \addplot [draw=none,fill=background,domain=-1:0] {-x} \closedcycle;
          \addplot [draw=none,fill=background,domain=2:3] {x-2} \closedcycle;
          \addplot [draw=none,fill=fillp,domain=0:1] {-x} \closedcycle;
          \addplot [draw=none,fill=fillp,domain=1:2] {x-2} \closedcycle;
          \addplot [draw=penColor,very thick,smooth] {-x};
          \addplot [draw=penColor2,very thick,smooth] {x-2};
          \addplot [draw=penColor3,very thick,smooth] {4+2*x-x^2};
         
        \end{axis}
\end{tikzpicture}
\end{image}
\end{hint}

\begin{hint}
	Next we find the $x$-coordinates of the relevant points of intersection.
	
	Let $a$ be the point of intersection between $y = -x$ and $y = 4+2x-x^2$, $b$ between $y=-x$ and $y=x-2$, and $c$ between $y=x-2$ and $y=4+2x-x^2$.

	Then
	
\[	
	\begin{cases}
		-a = 4+2a-a^2\\
		-b = b-2\\
		c-2 = 4+2c-c^2
	\end{cases}	
\]

\[	
	\begin{cases}
		0 = 4+3a-a^2\\
		 0 = 2b-2\\
		0= 6+c-c^2
	\end{cases}	
\]

\[	
	\begin{cases}
		0 = (1+a)(4-a)\\
		 b = 1\\
		0= (3-c)(2+c)
	\end{cases}	
\]

Thus $a=-1$,  $b = 1$, and $c = 3$ (make sure you understand why $a=4$ and $c=-2$ are not the correct intersections).
\end{hint}


\begin{hint}
	Thus the area of this region is

	\[
	\int_{-1}^{1} (4+2x-x^2) - (-x) \d x + \int_{1}^{3} (4+2x-x^2) - (x-2) \d x
	\]
\end{hint}

\begin{hint}
	The first summand is

	\begin{align*}
		\int_{-1}^{1} (4+2x-x^2) - (-x) \d x &=  \int_{-1}^{1} (4+3x-x^2) \d x\\
		&= \eval{4x+\frac{3}{2}x^2-\frac{1}{3}x^3}_{-1}^1\\
		&= \frac{22}{3}
	\end{align*}

	The second summand is

	\begin{align*}
		\int_{1}^{3} (4+2x-x^2) - (x-2) \d x &= \int_{1}^{3} (6+x-x^2) \d x\\
		&= \eval{6x+\frac{x^2}{2}-\frac{x^3}{3}}_1^3\\
		&= \frac{22}{3}
	\end{align*}

	Note that these two area equal, which we could have also discovered by observing the symmetry of the figure about the line $x=1$.
\end{hint}

\begin{prompt}
	\[
		\textrm{Area} = \answer{\frac{44}{3}}
	\]
\end{prompt}

\end{exercise}
\end{document}