\documentclass{ximera}

\input{preamble.tex}

\author{Matthew Carr}
%% BADBAD
%% From OSU 1151 Sample Exams
%% License?
%% Acknowledgement?
\license{BADBAD}
\acknowledgement{BADBAD}

\begin{document}
\begin{exercise}

\outcome{Calculate limits using the limit laws.}
\outcome{Calculate limits of the form 0/0.}

Find
\[
\lim_{x\to0}\left(\frac{\cos^{2}(x)-1}{\cos(x)-1}\right)
\begin{prompt}
= \answer{2}
\end{prompt}
\]

\begin{hint}
Recall that for any two numbers, $a$ and $b$,  $a^2-b^2=(a-b)(a+b)$. Factor the numerator of the expression in this manner.
\end{hint}
\begin{hint}
$\cos^{2}(x)-1=(\cos(x)-1)(\cos(x)+1)$ so $\frac{(\cos(x)-1)(\cos(x)+1)}{\cos(x)-1}=\cos(x)+1$ for $x\ne2\pi{n}$ for any integer $n$ (notice that if $x=2\pi n$, then $\cos(2\pi n)-1=0$ in the denominator) and $\lim_{x\to0}\left(\frac{\cos^{2}(x)-1}{\cos(x)-1}\right)=\lim_{x\to0}\left(\cos(x)+1\right)$ and this is $\lim_{x\to0}\left(\cos(x)\right)+\lim_{x\to0}\left(1\right)=2$.

\end{hint}
\end{exercise}
\end{document}